mod CLockTests
see ed527309

dartagnan/src/test/resources/locks/linuxrwlock-3-rel2rx.bpl
@@ -43,7 +43,7 @@ const $MALLOC_TOP: ref;
 var $M.0: [ref] i32;
 
 // Memory address bounds
-axiom ($GLOBALS_BOTTOM == $sub.ref(0, 36112));
+axiom ($GLOBALS_BOTTOM == $sub.ref(0, 36105));
 axiom ($EXTERNS_BOTTOM == $add.ref($GLOBALS_BOTTOM, $sub.ref(0, 32768)));
 axiom ($MALLOC_TOP == 9223372036854775807);
 function {:inline} $isExternal(p: ref) returns (bool) { $slt.ref.bool(p, $EXTERNS_BOTTOM) }
@@ -1491,37 +1491,16 @@ const mylock: ref;
 axiom (mylock == $sub.ref(0, 1028));
 const shareddata: ref;
 axiom (shareddata == $sub.ref(0, 2056));
-const assert_: ref;
-axiom (assert_ == $sub.ref(0, 3088));
-procedure  assert_($i0: i32)
-{
-$bb0:
-  assume {:sourceloc "include/assert.h", 2, 31} true;
-  assume {:verifier.code 1} true;
-  call {:cexpr "assert_:arg:exp"} boogie_si_record_i32($i0);
-  assume {:sourceloc "include/assert.h", 2, 31} true;
-  assume {:verifier.code 1} true;
-  call __VERIFIER_assert($i0);
-  assume {:sourceloc "include/assert.h", 2, 54} true;
-  assume {:verifier.code 0} true;
-  $exn := false;
-  return;
-}
-const llvm.dbg.declare: ref;
-axiom (llvm.dbg.declare == $sub.ref(0, 4120));
-procedure  llvm.dbg.declare($p0: ref, $p1: ref, $p2: ref);
-const __VERIFIER_assert: ref;
-axiom (__VERIFIER_assert == $sub.ref(0, 5152));
-procedure  __VERIFIER_assert($i0: i32);
+const .str: ref;
+axiom (.str == $sub.ref(0, 3081));
 const threadR: ref;
-axiom (threadR == $sub.ref(0, 6184));
+axiom (threadR == $sub.ref(0, 4113));
 procedure  threadR($p0: ref)
   returns ($r: ref)
 {
   var $i1: i32;
   var $i2: i32;
   var $i3: i1;
-  var $i4: i32;
 $bb0:
   assume {:sourceloc "benchmarks/locks/linuxrwlock-3-rel2rx.c", 133, 5} true;
   assume {:verifier.code 0} true;
@@ -1532,18 +1511,30 @@ $bb0:
   assume {:verifier.code 0} true;
   $i1 := $load.i32($M.0, shareddata);
   call {:cexpr "r"} boogie_si_record_i32($i1);
-  assume {:sourceloc "benchmarks/locks/linuxrwlock-3-rel2rx.c", 135, 17} true;
-  assume {:verifier.code 0} true;
-  $i2 := $load.i32($M.0, shareddata);
-  assume {:sourceloc "benchmarks/locks/linuxrwlock-3-rel2rx.c", 135, 14} true;
-  assume {:verifier.code 0} true;
-  $i3 := $eq.i32($i1, $i2);
-  assume {:sourceloc "benchmarks/locks/linuxrwlock-3-rel2rx.c", 135, 14} true;
-  assume {:verifier.code 0} true;
-  $i4 := $zext.i1.i32($i3);
   assume {:sourceloc "benchmarks/locks/linuxrwlock-3-rel2rx.c", 135, 5} true;
   assume {:verifier.code 0} true;
-  call assert_($i4);
+  $i2 := $load.i32($M.0, shareddata);
+  assume {:sourceloc "benchmarks/locks/linuxrwlock-3-rel2rx.c", 135, 5} true;
+  assume {:verifier.code 0} true;
+  $i3 := $eq.i32($i1, $i2);
+  assume {:sourceloc "benchmarks/locks/linuxrwlock-3-rel2rx.c", 135, 5} true;
+  assume {:verifier.code 0} true;
+  assume {:branchcond $i3} true;
+  goto $bb1, $bb2;
+$bb1:
+  assume ($i3 == 1);
+  assume {:sourceloc "benchmarks/locks/linuxrwlock-3-rel2rx.c", 135, 5} true;
+  assume {:verifier.code 0} true;
+  goto $bb3;
+$bb2:
+  assume !(($i3 == 1));
+  assume {:sourceloc "benchmarks/locks/linuxrwlock-3-rel2rx.c", 135, 5} true;
+  assume {:verifier.code 0} true;
+  call __assert_fail(.str, .str, 0, .str);
+  assume {:sourceloc "benchmarks/locks/linuxrwlock-3-rel2rx.c", 135, 5} true;
+  assume {:verifier.code 0} true;
+  goto $bb3;
+$bb3:
   assume {:sourceloc "benchmarks/locks/linuxrwlock-3-rel2rx.c", 136, 5} true;
   assume {:verifier.code 0} true;
   call read_unlock(mylock);
@@ -1553,8 +1544,11 @@ $bb0:
   $exn := false;
   return;
 }
+const llvm.dbg.declare: ref;
+axiom (llvm.dbg.declare == $sub.ref(0, 5145));
+procedure  llvm.dbg.declare($p0: ref, $p1: ref, $p2: ref);
 const read_lock: ref;
-axiom (read_lock == $sub.ref(0, 7216));
+axiom (read_lock == $sub.ref(0, 6177));
 procedure  read_lock($p0: ref)
 {
   var $p1: ref;
@@ -1642,8 +1636,11 @@ $bb6:
   $i3 := $i11;
   goto $bb1;
 }
+const __assert_fail: ref;
+axiom (__assert_fail == $sub.ref(0, 7209));
+procedure  __assert_fail($p0: ref, $p1: ref, $i2: i32, $p3: ref);
 const read_unlock: ref;
-axiom (read_unlock == $sub.ref(0, 8248));
+axiom (read_unlock == $sub.ref(0, 8241));
 procedure  read_unlock($p0: ref)
 {
   var $p1: ref;
@@ -1663,25 +1660,24 @@ $bb0:
   return;
 }
 const atomic_fetch_add_explicit: ref;
-axiom (atomic_fetch_add_explicit == $sub.ref(0, 9280));
+axiom (atomic_fetch_add_explicit == $sub.ref(0, 9273));
 procedure  atomic_fetch_add_explicit.ref.i32.i32(p.0: ref, p.1: i32, p.2: i32)
   returns ($r: i32);
 const atomic_fetch_sub_explicit: ref;
-axiom (atomic_fetch_sub_explicit == $sub.ref(0, 10312));
+axiom (atomic_fetch_sub_explicit == $sub.ref(0, 10305));
 procedure  atomic_fetch_sub_explicit.ref.i32.i32(p.0: ref, p.1: i32, p.2: i32)
   returns ($r: i32);
 const atomic_load_explicit: ref;
-axiom (atomic_load_explicit == $sub.ref(0, 11344));
+axiom (atomic_load_explicit == $sub.ref(0, 11337));
 procedure  atomic_load_explicit.ref.i32(p.0: ref, p.1: i32)
   returns ($r: i32);
 const threadW: ref;
-axiom (threadW == $sub.ref(0, 12376));
+axiom (threadW == $sub.ref(0, 12369));
 procedure  threadW($p0: ref)
   returns ($r: ref)
 {
   var $i1: i32;
   var $i2: i1;
-  var $i3: i32;
 $bb0:
   assume {:sourceloc "benchmarks/locks/linuxrwlock-3-rel2rx.c", 142, 5} true;
   assume {:verifier.code 0} true;
@@ -1692,18 +1688,30 @@ $bb0:
   assume {:verifier.code 0} true;
   $M.0 := $store.i32($M.0, shareddata, 42);
   call {:cexpr "shareddata"} boogie_si_record_i32(42);
-  assume {:sourceloc "benchmarks/locks/linuxrwlock-3-rel2rx.c", 144, 18} true;
-  assume {:verifier.code 0} true;
-  $i1 := $load.i32($M.0, shareddata);
-  assume {:sourceloc "benchmarks/locks/linuxrwlock-3-rel2rx.c", 144, 15} true;
-  assume {:verifier.code 0} true;
-  $i2 := $eq.i32(42, $i1);
-  assume {:sourceloc "benchmarks/locks/linuxrwlock-3-rel2rx.c", 144, 15} true;
-  assume {:verifier.code 0} true;
-  $i3 := $zext.i1.i32($i2);
   assume {:sourceloc "benchmarks/locks/linuxrwlock-3-rel2rx.c", 144, 5} true;
   assume {:verifier.code 0} true;
-  call assert_($i3);
+  $i1 := $load.i32($M.0, shareddata);
+  assume {:sourceloc "benchmarks/locks/linuxrwlock-3-rel2rx.c", 144, 5} true;
+  assume {:verifier.code 0} true;
+  $i2 := $eq.i32(42, $i1);
+  assume {:sourceloc "benchmarks/locks/linuxrwlock-3-rel2rx.c", 144, 5} true;
+  assume {:verifier.code 0} true;
+  assume {:branchcond $i2} true;
+  goto $bb1, $bb2;
+$bb1:
+  assume ($i2 == 1);
+  assume {:sourceloc "benchmarks/locks/linuxrwlock-3-rel2rx.c", 144, 5} true;
+  assume {:verifier.code 0} true;
+  goto $bb3;
+$bb2:
+  assume !(($i2 == 1));
+  assume {:sourceloc "benchmarks/locks/linuxrwlock-3-rel2rx.c", 144, 5} true;
+  assume {:verifier.code 0} true;
+  call __assert_fail(.str, .str, 0, .str);
+  assume {:sourceloc "benchmarks/locks/linuxrwlock-3-rel2rx.c", 144, 5} true;
+  assume {:verifier.code 0} true;
+  goto $bb3;
+$bb3:
   assume {:sourceloc "benchmarks/locks/linuxrwlock-3-rel2rx.c", 145, 5} true;
   assume {:verifier.code 0} true;
   call write_unlock(mylock);
@@ -1714,7 +1722,7 @@ $bb0:
   return;
 }
 const write_lock: ref;
-axiom (write_lock == $sub.ref(0, 13408));
+axiom (write_lock == $sub.ref(0, 13401));
 procedure  write_lock($p0: ref)
 {
   var $p1: ref;
@@ -1803,7 +1811,7 @@ $bb6:
   goto $bb1;
 }
 const write_unlock: ref;
-axiom (write_unlock == $sub.ref(0, 14440));
+axiom (write_unlock == $sub.ref(0, 14433));
 procedure  write_unlock($p0: ref)
 {
   var $p1: ref;
@@ -1823,7 +1831,7 @@ $bb0:
   return;
 }
 const threadRW: ref;
-axiom (threadRW == $sub.ref(0, 15472));
+axiom (threadRW == $sub.ref(0, 15465));
 procedure  threadRW($p0: ref)
   returns ($r: ref)
 {
@@ -1835,10 +1843,8 @@ procedure  threadRW($p0: ref)
   var $i6: i32;
   var $i7: i1;
   var $i8: i32;
-  var $i9: i32;
-  var $i10: i1;
-  var $i11: i32;
-  var $i12: i32;
+  var $i9: i1;
+  var $i10: i32;
 $bb0:
   assume {:sourceloc "benchmarks/locks/linuxrwlock-3-rel2rx.c", 151, 10} true;
   assume {:verifier.code 0} true;
@@ -1884,24 +1890,16 @@ $bb4:
   assume {:verifier.code 0} true;
   $i5 := $load.i32($M.0, shareddata);
   call {:cexpr "r"} boogie_si_record_i32($i5);
-  assume {:sourceloc "benchmarks/locks/linuxrwlock-3-rel2rx.c", 155, 25} true;
-  assume {:verifier.code 0} true;
-  $i6 := $load.i32($M.0, shareddata);
-  assume {:sourceloc "benchmarks/locks/linuxrwlock-3-rel2rx.c", 155, 22} true;
-  assume {:verifier.code 0} true;
-  $i7 := $eq.i32($i5, $i6);
-  assume {:sourceloc "benchmarks/locks/linuxrwlock-3-rel2rx.c", 155, 22} true;
-  assume {:verifier.code 0} true;
-  $i8 := $zext.i1.i32($i7);
   assume {:sourceloc "benchmarks/locks/linuxrwlock-3-rel2rx.c", 155, 13} true;
   assume {:verifier.code 0} true;
-  call assert_($i8);
-  assume {:sourceloc "benchmarks/locks/linuxrwlock-3-rel2rx.c", 156, 13} true;
+  $i6 := $load.i32($M.0, shareddata);
+  assume {:sourceloc "benchmarks/locks/linuxrwlock-3-rel2rx.c", 155, 13} true;
   assume {:verifier.code 0} true;
-  call read_unlock(mylock);
-  assume {:sourceloc "benchmarks/locks/linuxrwlock-3-rel2rx.c", 157, 9} true;
+  $i7 := $eq.i32($i5, $i6);
+  assume {:sourceloc "benchmarks/locks/linuxrwlock-3-rel2rx.c", 155, 13} true;
   assume {:verifier.code 0} true;
-  goto $bb6;
+  assume {:branchcond $i7} true;
+  goto $bb6, $bb7;
 $bb5:
   assume !(($i4 == 1));
   assume {:sourceloc "benchmarks/locks/linuxrwlock-3-rel2rx.c", 158, 13} true;
@@ -1911,39 +1909,71 @@ $bb5:
   assume {:verifier.code 0} true;
   $M.0 := $store.i32($M.0, shareddata, $i1);
   call {:cexpr "shareddata"} boogie_si_record_i32($i1);
-  assume {:sourceloc "benchmarks/locks/linuxrwlock-3-rel2rx.c", 160, 20} true;
-  assume {:verifier.code 0} true;
-  $i9 := $load.i32($M.0, shareddata);
-  assume {:sourceloc "benchmarks/locks/linuxrwlock-3-rel2rx.c", 160, 31} true;
-  assume {:verifier.code 0} true;
-  $i10 := $eq.i32($i9, $i1);
-  assume {:sourceloc "benchmarks/locks/linuxrwlock-3-rel2rx.c", 160, 31} true;
-  assume {:verifier.code 0} true;
-  $i11 := $zext.i1.i32($i10);
   assume {:sourceloc "benchmarks/locks/linuxrwlock-3-rel2rx.c", 160, 13} true;
   assume {:verifier.code 0} true;
-  call assert_($i11);
+  $i8 := $load.i32($M.0, shareddata);
+  assume {:sourceloc "benchmarks/locks/linuxrwlock-3-rel2rx.c", 160, 13} true;
+  assume {:verifier.code 0} true;
+  $i9 := $eq.i32($i8, $i1);
+  assume {:sourceloc "benchmarks/locks/linuxrwlock-3-rel2rx.c", 160, 13} true;
+  assume {:verifier.code 0} true;
+  assume {:branchcond $i9} true;
+  goto $bb10, $bb11;
+$bb6:
+  assume ($i7 == 1);
+  assume {:sourceloc "benchmarks/locks/linuxrwlock-3-rel2rx.c", 155, 13} true;
+  assume {:verifier.code 0} true;
+  goto $bb8;
+$bb7:
+  assume !(($i7 == 1));
+  assume {:sourceloc "benchmarks/locks/linuxrwlock-3-rel2rx.c", 155, 13} true;
+  assume {:verifier.code 0} true;
+  call __assert_fail(.str, .str, 0, .str);
+  assume {:sourceloc "benchmarks/locks/linuxrwlock-3-rel2rx.c", 155, 13} true;
+  assume {:verifier.code 0} true;
+  goto $bb8;
+$bb8:
+  assume {:sourceloc "benchmarks/locks/linuxrwlock-3-rel2rx.c", 156, 13} true;
+  assume {:verifier.code 0} true;
+  call read_unlock(mylock);
+  assume {:sourceloc "benchmarks/locks/linuxrwlock-3-rel2rx.c", 157, 9} true;
+  assume {:verifier.code 0} true;
+  goto $bb9;
+$bb9:
+  assume {:sourceloc "benchmarks/locks/linuxrwlock-3-rel2rx.c", 163, 5} true;
+  assume {:verifier.code 0} true;
+  goto $bb13;
+$bb10:
+  assume ($i9 == 1);
+  assume {:sourceloc "benchmarks/locks/linuxrwlock-3-rel2rx.c", 160, 13} true;
+  assume {:verifier.code 0} true;
+  goto $bb12;
+$bb11:
+  assume !(($i9 == 1));
+  assume {:sourceloc "benchmarks/locks/linuxrwlock-3-rel2rx.c", 160, 13} true;
+  assume {:verifier.code 0} true;
+  call __assert_fail(.str, .str, 0, .str);
+  assume {:sourceloc "benchmarks/locks/linuxrwlock-3-rel2rx.c", 160, 13} true;
+  assume {:verifier.code 0} true;
+  goto $bb12;
+$bb12:
   assume {:sourceloc "benchmarks/locks/linuxrwlock-3-rel2rx.c", 161, 13} true;
   assume {:verifier.code 0} true;
   call write_unlock(mylock);
   assume {:verifier.code 0} true;
-  goto $bb6;
-$bb6:
-  assume {:sourceloc "benchmarks/locks/linuxrwlock-3-rel2rx.c", 163, 5} true;
-  assume {:verifier.code 0} true;
-  goto $bb7;
-$bb7:
+  goto $bb9;
+$bb13:
   assume {:sourceloc "benchmarks/locks/linuxrwlock-3-rel2rx.c", 151, 29} true;
   assume {:verifier.code 0} true;
-  $i12 := $add.i32($i1, 1);
-  call {:cexpr "i"} boogie_si_record_i32($i12);
+  $i10 := $add.i32($i1, 1);
+  call {:cexpr "i"} boogie_si_record_i32($i10);
   assume {:sourceloc "benchmarks/locks/linuxrwlock-3-rel2rx.c", 151, 5} true;
   assume {:verifier.code 0} true;
-  $i1 := $i12;
+  $i1 := $i10;
   goto $bb1;
 }
 const main: ref;
-axiom (main == $sub.ref(0, 16504));
+axiom (main == $sub.ref(0, 16497));
 procedure {:entrypoint} main()
   returns ($r: i32)
 {
@@ -1987,19 +2017,19 @@ $bb0:
   return;
 }
 const atomic_init: ref;
-axiom (atomic_init == $sub.ref(0, 17536));
+axiom (atomic_init == $sub.ref(0, 17529));
 procedure  atomic_init.ref.i32(p.0: ref, p.1: i32)
   returns ($r: i32);
 const pthread_create: ref;
-axiom (pthread_create == $sub.ref(0, 18568));
+axiom (pthread_create == $sub.ref(0, 18561));
 procedure  pthread_create($p0: ref, $p1: ref, $p2: ref, $p3: ref)
   returns ($r: i32);
 const __SMACK_code: ref;
-axiom (__SMACK_code == $sub.ref(0, 19600));
+axiom (__SMACK_code == $sub.ref(0, 19593));
 procedure  __SMACK_code.ref($p0: ref);
 procedure  __SMACK_code.ref.i32($p0: ref, p.1: i32);
 const __VERIFIER_assume: ref;
-axiom (__VERIFIER_assume == $sub.ref(0, 20632));
+axiom (__VERIFIER_assume == $sub.ref(0, 20625));
 procedure  __VERIFIER_assume($i0: i32)
 {
 $bb0:
@@ -2018,7 +2048,7 @@ $bb0:
   return;
 }
 const __SMACK_dummy: ref;
-axiom (__SMACK_dummy == $sub.ref(0, 21664));
+axiom (__SMACK_dummy == $sub.ref(0, 21657));
 procedure  __SMACK_dummy($i0: i32)
 {
 $bb0:
@@ -2034,7 +2064,7 @@ $bb0:
   return;
 }
 const __SMACK_and32: ref;
-axiom (__SMACK_and32 == $sub.ref(0, 22696));
+axiom (__SMACK_and32 == $sub.ref(0, 22689));
 procedure  __SMACK_and32($i0: i32, $i1: i32)
   returns ($r: i32)
 {
@@ -9246,7 +9276,7 @@ $bb576:
   goto $bb570;
 }
 const __SMACK_and64: ref;
-axiom (__SMACK_and64 == $sub.ref(0, 23728));
+axiom (__SMACK_and64 == $sub.ref(0, 23721));
 procedure  __SMACK_and64($i0: i64, $i1: i64)
   returns ($r: i64)
 {
@@ -9279,7 +9309,7 @@ $bb0:
   return;
 }
 const __SMACK_and16: ref;
-axiom (__SMACK_and16 == $sub.ref(0, 24760));
+axiom (__SMACK_and16 == $sub.ref(0, 24753));
 procedure  __SMACK_and16($i0: i16, $i1: i16)
   returns ($r: i16)
 {
@@ -11939,7 +11969,7 @@ $bb144:
   goto $bb138;
 }
 const __SMACK_and8: ref;
-axiom (__SMACK_and8 == $sub.ref(0, 25792));
+axiom (__SMACK_and8 == $sub.ref(0, 25785));
 procedure  __SMACK_and8($i0: i8, $i1: i8)
   returns ($r: i8)
 {
@@ -13247,7 +13277,7 @@ $bb72:
   goto $bb66;
 }
 const __SMACK_or32: ref;
-axiom (__SMACK_or32 == $sub.ref(0, 26824));
+axiom (__SMACK_or32 == $sub.ref(0, 26817));
 procedure  __SMACK_or32($i0: i32, $i1: i32)
   returns ($r: i32)
 {
@@ -16363,7 +16393,7 @@ $bb192:
   goto $bb189;
 }
 const __SMACK_or64: ref;
-axiom (__SMACK_or64 == $sub.ref(0, 27856));
+axiom (__SMACK_or64 == $sub.ref(0, 27849));
 procedure  __SMACK_or64($i0: i64, $i1: i64)
   returns ($r: i64)
 {
@@ -16396,7 +16426,7 @@ $bb0:
   return;
 }
 const __SMACK_or16: ref;
-axiom (__SMACK_or16 == $sub.ref(0, 28888));
+axiom (__SMACK_or16 == $sub.ref(0, 28881));
 procedure  __SMACK_or16($i0: i16, $i1: i16)
   returns ($r: i16)
 {
@@ -16429,7 +16459,7 @@ $bb0:
   return;
 }
 const __SMACK_or8: ref;
-axiom (__SMACK_or8 == $sub.ref(0, 29920));
+axiom (__SMACK_or8 == $sub.ref(0, 29913));
 procedure  __SMACK_or8($i0: i8, $i1: i8)
   returns ($r: i8)
 {
@@ -16462,7 +16492,7 @@ $bb0:
   return;
 }
 const __SMACK_check_overflow: ref;
-axiom (__SMACK_check_overflow == $sub.ref(0, 30952));
+axiom (__SMACK_check_overflow == $sub.ref(0, 30945));
 procedure  __SMACK_check_overflow($i0: i32)
 {
 $bb0:
@@ -16481,7 +16511,7 @@ $bb0:
   return;
 }
 const __SMACK_decls: ref;
-axiom (__SMACK_decls == $sub.ref(0, 31984));
+axiom (__SMACK_decls == $sub.ref(0, 31977));
 type $mop;
 procedure  boogie_si_record_mop(m: $mop);
 const $MOP: $mop;
@@ -16520,10 +16550,10 @@ modifies $CurrAddr;
 procedure  $free(p: ref);
 
 const __SMACK_top_decl: ref;
-axiom (__SMACK_top_decl == $sub.ref(0, 33016));
+axiom (__SMACK_top_decl == $sub.ref(0, 33009));
 procedure  __SMACK_top_decl.ref($p0: ref);
 const __SMACK_init_func_memory_model: ref;
-axiom (__SMACK_init_func_memory_model == $sub.ref(0, 34048));
+axiom (__SMACK_init_func_memory_model == $sub.ref(0, 34041));
 procedure  __SMACK_init_func_memory_model()
 {
 $bb0:
@@ -16538,10 +16568,10 @@ $bb0:
   return;
 }
 const llvm.dbg.value: ref;
-axiom (llvm.dbg.value == $sub.ref(0, 35080));
+axiom (llvm.dbg.value == $sub.ref(0, 35073));
 procedure  llvm.dbg.value($p0: ref, $p1: ref, $p2: ref);
 const __SMACK_static_init: ref;
-axiom (__SMACK_static_init == $sub.ref(0, 36112));
+axiom (__SMACK_static_init == $sub.ref(0, 36105));
 procedure  __SMACK_static_init()
 {
 $bb0:
