dartagnan/src/test/resources/locks/mutex_musl-3.bpl
@@ -43,7 +43,7 @@ const $MALLOC_TOP: ref;
 var $M.0: [ref] i8;
 
 // Memory address bounds
-axiom ($GLOBALS_BOTTOM == $sub.ref(0, 42304));
+axiom ($GLOBALS_BOTTOM == $sub.ref(0, 42297));
 axiom ($EXTERNS_BOTTOM == $add.ref($GLOBALS_BOTTOM, $sub.ref(0, 32768)));
 axiom ($MALLOC_TOP == 9223372036854775807);
 function {:inline} $isExternal(p: ref) returns (bool) { $slt.ref.bool(p, $EXTERNS_BOTTOM) }
@@ -1491,32 +1491,12 @@ const mutex: ref;
 axiom (mutex == $sub.ref(0, 1032));
 const shared: ref;
 axiom (shared == $sub.ref(0, 2060));
+const .str: ref;
+axiom (.str == $sub.ref(0, 3085));
 const sig: ref;
-axiom (sig == $sub.ref(0, 3088));
-const assert_: ref;
-axiom (assert_ == $sub.ref(0, 4120));
-procedure  assert_($i0: i32)
-{
-$bb0:
-  assume {:sourceloc "include/assert.h", 2, 31} true;
-  assume {:verifier.code 1} true;
-  call {:cexpr "assert_:arg:exp"} boogie_si_record_i32($i0);
-  assume {:sourceloc "include/assert.h", 2, 31} true;
-  assume {:verifier.code 1} true;
-  call __VERIFIER_assert($i0);
-  assume {:sourceloc "include/assert.h", 2, 54} true;
-  assume {:verifier.code 0} true;
-  $exn := false;
-  return;
-}
-const llvm.dbg.declare: ref;
-axiom (llvm.dbg.declare == $sub.ref(0, 5152));
-procedure  llvm.dbg.declare($p0: ref, $p1: ref, $p2: ref);
-const __VERIFIER_assert: ref;
-axiom (__VERIFIER_assert == $sub.ref(0, 6184));
-procedure  __VERIFIER_assert($i0: i32);
+axiom (sig == $sub.ref(0, 4113));
 const thread_n: ref;
-axiom (thread_n == $sub.ref(0, 7216));
+axiom (thread_n == $sub.ref(0, 5145));
 procedure  thread_n($p0: ref)
   returns ($r: ref)
 {
@@ -1526,8 +1506,7 @@ procedure  thread_n($p0: ref)
   var $i4: i32;
   var $i5: i64;
   var $i6: i1;
-  var $i7: i32;
-  var $p8: ref;
+  var $p7: ref;
 $bb0:
   assume {:sourceloc "benchmarks/locks/mutex_musl-3.c", 99, 23} true;
   assume {:verifier.code 0} true;
@@ -1552,32 +1531,47 @@ $bb0:
   assume {:verifier.code 0} true;
   $i4 := $load.i32($M.0, shared);
   call {:cexpr "r"} boogie_si_record_i32($i4);
-  assume {:sourceloc "benchmarks/locks/mutex_musl-3.c", 104, 12} true;
-  assume {:verifier.code 0} true;
-  $i5 := $sext.i32.i64($i4);
-  assume {:sourceloc "benchmarks/locks/mutex_musl-3.c", 104, 14} true;
-  assume {:verifier.code 0} true;
-  $i6 := $eq.i64($i5, $i1);
-  assume {:sourceloc "benchmarks/locks/mutex_musl-3.c", 104, 14} true;
-  assume {:verifier.code 0} true;
-  $i7 := $zext.i1.i32($i6);
   assume {:sourceloc "benchmarks/locks/mutex_musl-3.c", 104, 5} true;
   assume {:verifier.code 0} true;
-  call assert_($i7);
+  $i5 := $sext.i32.i64($i4);
+  assume {:sourceloc "benchmarks/locks/mutex_musl-3.c", 104, 5} true;
+  assume {:verifier.code 0} true;
+  $i6 := $eq.i64($i5, $i1);
+  assume {:sourceloc "benchmarks/locks/mutex_musl-3.c", 104, 5} true;
+  assume {:verifier.code 0} true;
+  assume {:branchcond $i6} true;
+  goto $bb1, $bb2;
+$bb1:
+  assume ($i6 == 1);
+  assume {:sourceloc "benchmarks/locks/mutex_musl-3.c", 104, 5} true;
+  assume {:verifier.code 0} true;
+  goto $bb3;
+$bb2:
+  assume !(($i6 == 1));
+  assume {:sourceloc "benchmarks/locks/mutex_musl-3.c", 104, 5} true;
+  assume {:verifier.code 0} true;
+  call __assert_fail(.str, .str, 0, .str);
+  assume {:sourceloc "benchmarks/locks/mutex_musl-3.c", 104, 5} true;
+  assume {:verifier.code 0} true;
+  goto $bb3;
+$bb3:
   assume {:sourceloc "benchmarks/locks/mutex_musl-3.c", 105, 18} true;
   assume {:verifier.code 0} true;
-  $p8 := $load.ref($M.0, mutex);
+  $p7 := $load.ref($M.0, mutex);
   assume {:sourceloc "benchmarks/locks/mutex_musl-3.c", 105, 5} true;
   assume {:verifier.code 0} true;
-  call mutex_unlock($p8);
+  call mutex_unlock($p7);
   assume {:sourceloc "benchmarks/locks/mutex_musl-3.c", 106, 5} true;
   assume {:verifier.code 0} true;
   $r := $0.ref;
   $exn := false;
   return;
 }
+const llvm.dbg.declare: ref;
+axiom (llvm.dbg.declare == $sub.ref(0, 6177));
+procedure  llvm.dbg.declare($p0: ref, $p1: ref, $p2: ref);
 const mutex_lock: ref;
-axiom (mutex_lock == $sub.ref(0, 8248));
+axiom (mutex_lock == $sub.ref(0, 7209));
 procedure  mutex_lock($p0: ref)
 {
   var $p1: ref;
@@ -1703,8 +1697,11 @@ $bb9:
   assume {:verifier.code 0} true;
   goto $bb8;
 }
+const __assert_fail: ref;
+axiom (__assert_fail == $sub.ref(0, 8241));
+procedure  __assert_fail($p0: ref, $p1: ref, $i2: i32, $p3: ref);
 const mutex_unlock: ref;
-axiom (mutex_unlock == $sub.ref(0, 9280));
+axiom (mutex_unlock == $sub.ref(0, 9273));
 procedure  mutex_unlock($p0: ref)
 {
   var $p1: ref;
@@ -1778,15 +1775,15 @@ $bb6:
   return;
 }
 const atomic_exchange_explicit: ref;
-axiom (atomic_exchange_explicit == $sub.ref(0, 10312));
+axiom (atomic_exchange_explicit == $sub.ref(0, 10305));
 procedure  atomic_exchange_explicit.ref.i32.i32(p.0: ref, p.1: i32, p.2: i32)
   returns ($r: i32);
 const atomic_load_explicit: ref;
-axiom (atomic_load_explicit == $sub.ref(0, 11344));
+axiom (atomic_load_explicit == $sub.ref(0, 11337));
 procedure  atomic_load_explicit.ref.i32(p.0: ref, p.1: i32)
   returns ($r: i32);
 const __futex_wake: ref;
-axiom (__futex_wake == $sub.ref(0, 12376));
+axiom (__futex_wake == $sub.ref(0, 12369));
 procedure  __futex_wake($p0: ref, $i1: i32)
 {
   var $i2: i32;
@@ -1803,11 +1800,11 @@ $bb0:
   return;
 }
 const atomic_fetch_add_explicit: ref;
-axiom (atomic_fetch_add_explicit == $sub.ref(0, 13408));
+axiom (atomic_fetch_add_explicit == $sub.ref(0, 13401));
 procedure  atomic_fetch_add_explicit.ref.i32.i32(p.0: ref, p.1: i32, p.2: i32)
   returns ($r: i32);
 const mutex_lock_fastpath: ref;
-axiom (mutex_lock_fastpath == $sub.ref(0, 14440));
+axiom (mutex_lock_fastpath == $sub.ref(0, 14433));
 procedure  mutex_lock_fastpath($p0: ref)
   returns ($r: i32)
 {
@@ -1836,11 +1833,11 @@ $bb0:
   return;
 }
 const atomic_thread_fence: ref;
-axiom (atomic_thread_fence == $sub.ref(0, 15472));
+axiom (atomic_thread_fence == $sub.ref(0, 15465));
 procedure  atomic_thread_fence.i32(p.0: i32)
   returns ($r: i32);
 const mutex_lock_slowpath_check: ref;
-axiom (mutex_lock_slowpath_check == $sub.ref(0, 16504));
+axiom (mutex_lock_slowpath_check == $sub.ref(0, 16497));
 procedure  mutex_lock_slowpath_check($p0: ref)
   returns ($r: i32)
 {
@@ -1869,11 +1866,11 @@ $bb0:
   return;
 }
 const atomic_compare_exchange_strong_explicit: ref;
-axiom (atomic_compare_exchange_strong_explicit == $sub.ref(0, 17536));
+axiom (atomic_compare_exchange_strong_explicit == $sub.ref(0, 17529));
 procedure  atomic_compare_exchange_strong_explicit.ref.ref.i32.i32.i32(p.0: ref, p.1: ref, p.2: i32, p.3: i32, p.4: i32)
   returns ($r: i32);
 const __futex_wait: ref;
-axiom (__futex_wait == $sub.ref(0, 18568));
+axiom (__futex_wait == $sub.ref(0, 18561));
 procedure  __futex_wait($p0: ref, $i1: i32)
 {
   var $i2: i32;
@@ -1937,11 +1934,11 @@ $bb6:
   goto $bb3;
 }
 const atomic_fetch_sub_explicit: ref;
-axiom (atomic_fetch_sub_explicit == $sub.ref(0, 19600));
+axiom (atomic_fetch_sub_explicit == $sub.ref(0, 19593));
 procedure  atomic_fetch_sub_explicit.ref.i32.i32(p.0: ref, p.1: i32, p.2: i32)
   returns ($r: i32);
 const main: ref;
-axiom (main == $sub.ref(0, 20632));
+axiom (main == $sub.ref(0, 20625));
 procedure {:entrypoint} main()
   returns ($r: i32)
 {
@@ -1999,14 +1996,14 @@ $bb0:
   return;
 }
 const malloc: ref;
-axiom (malloc == $sub.ref(0, 21664));
+axiom (malloc == $sub.ref(0, 21657));
 procedure  malloc($i0: i64)
   returns ($r: ref)
 {
   call $r := $malloc($i0);
 }
 const mutex_init: ref;
-axiom (mutex_init == $sub.ref(0, 22696));
+axiom (mutex_init == $sub.ref(0, 22689));
 procedure  mutex_init($p0: ref)
 {
   var $p1: ref;
@@ -2034,19 +2031,19 @@ $bb0:
   return;
 }
 const pthread_create: ref;
-axiom (pthread_create == $sub.ref(0, 23728));
+axiom (pthread_create == $sub.ref(0, 23721));
 procedure  pthread_create($p0: ref, $p1: ref, $p2: ref, $p3: ref)
   returns ($r: i32);
 const atomic_init: ref;
-axiom (atomic_init == $sub.ref(0, 24760));
+axiom (atomic_init == $sub.ref(0, 24753));
 procedure  atomic_init.ref.i32(p.0: ref, p.1: i32)
   returns ($r: i32);
 const __SMACK_code: ref;
-axiom (__SMACK_code == $sub.ref(0, 25792));
+axiom (__SMACK_code == $sub.ref(0, 25785));
 procedure  __SMACK_code.ref($p0: ref);
 procedure  __SMACK_code.ref.i32($p0: ref, p.1: i32);
 const __VERIFIER_assume: ref;
-axiom (__VERIFIER_assume == $sub.ref(0, 26824));
+axiom (__VERIFIER_assume == $sub.ref(0, 26817));
 procedure  __VERIFIER_assume($i0: i32)
 {
 $bb0:
@@ -2065,7 +2062,7 @@ $bb0:
   return;
 }
 const __SMACK_dummy: ref;
-axiom (__SMACK_dummy == $sub.ref(0, 27856));
+axiom (__SMACK_dummy == $sub.ref(0, 27849));
 procedure  __SMACK_dummy($i0: i32)
 {
 $bb0:
@@ -2081,7 +2078,7 @@ $bb0:
   return;
 }
 const __SMACK_and32: ref;
-axiom (__SMACK_and32 == $sub.ref(0, 28888));
+axiom (__SMACK_and32 == $sub.ref(0, 28881));
 procedure  __SMACK_and32($i0: i32, $i1: i32)
   returns ($r: i32)
 {
@@ -9293,7 +9290,7 @@ $bb576:
   goto $bb570;
 }
 const __SMACK_and64: ref;
-axiom (__SMACK_and64 == $sub.ref(0, 29920));
+axiom (__SMACK_and64 == $sub.ref(0, 29913));
 procedure  __SMACK_and64($i0: i64, $i1: i64)
   returns ($r: i64)
 {
@@ -9326,7 +9323,7 @@ $bb0:
   return;
 }
 const __SMACK_and16: ref;
-axiom (__SMACK_and16 == $sub.ref(0, 30952));
+axiom (__SMACK_and16 == $sub.ref(0, 30945));
 procedure  __SMACK_and16($i0: i16, $i1: i16)
   returns ($r: i16)
 {
@@ -11986,7 +11983,7 @@ $bb144:
   goto $bb138;
 }
 const __SMACK_and8: ref;
-axiom (__SMACK_and8 == $sub.ref(0, 31984));
+axiom (__SMACK_and8 == $sub.ref(0, 31977));
 procedure  __SMACK_and8($i0: i8, $i1: i8)
   returns ($r: i8)
 {
@@ -13294,7 +13291,7 @@ $bb72:
   goto $bb66;
 }
 const __SMACK_or32: ref;
-axiom (__SMACK_or32 == $sub.ref(0, 33016));
+axiom (__SMACK_or32 == $sub.ref(0, 33009));
 procedure  __SMACK_or32($i0: i32, $i1: i32)
   returns ($r: i32)
 {
@@ -16410,7 +16407,7 @@ $bb192:
   goto $bb189;
 }
 const __SMACK_or64: ref;
-axiom (__SMACK_or64 == $sub.ref(0, 34048));
+axiom (__SMACK_or64 == $sub.ref(0, 34041));
 procedure  __SMACK_or64($i0: i64, $i1: i64)
   returns ($r: i64)
 {
@@ -16443,7 +16440,7 @@ $bb0:
   return;
 }
 const __SMACK_or16: ref;
-axiom (__SMACK_or16 == $sub.ref(0, 35080));
+axiom (__SMACK_or16 == $sub.ref(0, 35073));
 procedure  __SMACK_or16($i0: i16, $i1: i16)
   returns ($r: i16)
 {
@@ -16476,7 +16473,7 @@ $bb0:
   return;
 }
 const __SMACK_or8: ref;
-axiom (__SMACK_or8 == $sub.ref(0, 36112));
+axiom (__SMACK_or8 == $sub.ref(0, 36105));
 procedure  __SMACK_or8($i0: i8, $i1: i8)
   returns ($r: i8)
 {
@@ -16509,7 +16506,7 @@ $bb0:
   return;
 }
 const __SMACK_check_overflow: ref;
-axiom (__SMACK_check_overflow == $sub.ref(0, 37144));
+axiom (__SMACK_check_overflow == $sub.ref(0, 37137));
 procedure  __SMACK_check_overflow($i0: i32)
 {
 $bb0:
@@ -16528,7 +16525,7 @@ $bb0:
   return;
 }
 const __SMACK_decls: ref;
-axiom (__SMACK_decls == $sub.ref(0, 38176));
+axiom (__SMACK_decls == $sub.ref(0, 38169));
 type $mop;
 procedure  boogie_si_record_mop(m: $mop);
 const $MOP: $mop;
@@ -16567,10 +16564,10 @@ modifies $CurrAddr;
 procedure  $free(p: ref);
 
 const __SMACK_top_decl: ref;
-axiom (__SMACK_top_decl == $sub.ref(0, 39208));
+axiom (__SMACK_top_decl == $sub.ref(0, 39201));
 procedure  __SMACK_top_decl.ref($p0: ref);
 const __SMACK_init_func_memory_model: ref;
-axiom (__SMACK_init_func_memory_model == $sub.ref(0, 40240));
+axiom (__SMACK_init_func_memory_model == $sub.ref(0, 40233));
 procedure  __SMACK_init_func_memory_model()
 {
 $bb0:
@@ -16585,10 +16582,10 @@ $bb0:
   return;
 }
 const llvm.dbg.value: ref;
-axiom (llvm.dbg.value == $sub.ref(0, 41272));
+axiom (llvm.dbg.value == $sub.ref(0, 41265));
 procedure  llvm.dbg.value($p0: ref, $p1: ref, $p2: ref);
 const __SMACK_static_init: ref;
-axiom (__SMACK_static_init == $sub.ref(0, 42304));
+axiom (__SMACK_static_init == $sub.ref(0, 42297));
 procedure  __SMACK_static_init()
 {
 $bb0:
